{
 "cells": [
  {
   "cell_type": "markdown",
   "metadata": {},
   "source": [
    "1. Find the value of T(2) for the recurrence relation T(n) = 3T(n-1) + 12n, given that T(0)=5."
   ]
  },
  {
   "cell_type": "code",
   "execution_count": 2,
   "metadata": {},
   "outputs": [],
   "source": [
    " ##To find the value of T(2) for the recurrence relation T(n)=3T(n-1) + 12n ,with\n",
    "#the initial condition T(0) = 5, we can use the recurrence relation iteratively.\n",
    " #                             T(1) = 3T(0) + 12(1)\n",
    " #                                  = 3(5)  + 12\n",
    " #                                  = 15  + 12 \n",
    " #                                  = 27\n",
    "\n",
    "#s let's find T(2):\n",
    "#                              T(2) = 3T(1) + 12(2)\n",
    "#                                   = 3(27) + 24\n",
    "#                                   = 81 + 24\n",
    "#                                   = 105\n",
    "#Therfore, the value of T(2) for the given recurrence relation is 105 \"\"\"                                  \n",
    "\n",
    "                              "
   ]
  },
  {
   "cell_type": "markdown",
   "metadata": {},
   "source": [
    "2. Given a recurrence relation, solve it using the substitution method:\n",
    "\n",
    "(a). T(n) = T(n-1) + c\n"
   ]
  },
  {
   "cell_type": "code",
   "execution_count": 6,
   "metadata": {},
   "outputs": [],
   "source": [
    "#To solve the recurrence relation T(n)=T(n−1)+c using the substitution method, let's express it in terms of smaller subproblems until we reach the base case.\n",
    "#The recurrence relation is:\n",
    "#                    T(n)=T(n−1)+c\n",
    "#s, let's expand it:\n",
    "#                    T(n)=T(n−2)+c+c\n",
    "#                    T(n)=T(n−3)+c+c+c\n",
    "#Continuing this pattern, we can express T(n) in terms of T(n−k) as:\n",
    "#                    T(n)=T(n−k)+k⋅c\n",
    "#We continue until we reach the base case, which is when n−k=0, or k=n:\n",
    " #                   T(n)=T(0)+n⋅c\n",
    "#s, substitute the base case T(0) with its given value:\n",
    "#                    T(n)=T(0)+n⋅c\n",
    "#Since T(0) is given as an initial condition, you can substitute the specific value to get the final solution.\n",
    "#For example, if T(0)=5, the solution is:\n",
    " #                   T(n)=5+n⋅c\n",
    "#So, the solution to the recurrence relation T(n)=T(n−1)+c using the substitution method is T(n)=5+n⋅c, where c is a constant.\n",
    "\n",
    "\n",
    "\n",
    "\n",
    "\n",
    "\n"
   ]
  },
  {
   "cell_type": "markdown",
   "metadata": {},
   "source": [
    "  2. Given a recurrence relation, solve it using the substitution method:\n",
    "  \n",
    "  b. T(n) = 2T(n/2) + n"
   ]
  },
  {
   "cell_type": "code",
   "execution_count": 9,
   "metadata": {},
   "outputs": [],
   "source": [
    "#To solve the recurrence relation T(n)= 2T(n/2)+n using the substitution method, we'll use repeated substitution and look for a pattern.\n",
    "#First Substitution:\n",
    "#             T(n)=2T(n/2)+n \n",
    "#Second Substitution:\n",
    "#             T(n/2)=2T(n/4)+n/2\n",
    "#Substitute this back into the original equation:\n",
    "\n",
    "#             T(n)=2(2T(n/4)+n/2\n",
    "#Simplify:\n",
    "#             T(n)=4T(n/4)+2n\n",
    "#Third Substitution:\n",
    "#             T(n/4)=2T(n/8)+n/4\n",
    " #Substitute this into the second substitution:\n",
    "#             T(n)=4(2T(n/8)+(n/4))+2n\n",
    "#Simplify:\n",
    "\n",
    "#             T(n)=8T(n/8)+3n\n",
    "\n",
    "#After k steps, we get:\n",
    "#            T(n)=2T(n/2k)+kn\n",
    "\n",
    "#s, we need to find the value of k when n/2k = 1, which gives us k=log2n.\n",
    "\n",
    "#Substitute k=log2n into the expression: \n",
    "             #T(n)= 2log2nT(1) + nlog2n\n",
    "\n",
    "#Simplify further using the fact that \n",
    "\n",
    "#             T(n)=nT(1)+nlog \n",
    "\n",
    "#If you have an initial condition T(1), you can substitute it in. If not, you can leave the solution in this form.\n"
   ]
  },
  {
   "cell_type": "markdown",
   "metadata": {},
   "source": [
    "2. Given a recurrence relation, solve it using the substitution method:\n",
    "\n",
    "c. T(n) = 2T(n/2) + c"
   ]
  },
  {
   "cell_type": "code",
   "execution_count": 10,
   "metadata": {},
   "outputs": [],
   "source": [
    "#To solve the recurrence relation T(n)= 2T(n/2)+c using the substitution method, we'll use repeated substitution and look for a pattern.\n",
    "#First Substitution:\n",
    "#             T(n)=2T(n/2)+c \n",
    "#Second Substitution:\n",
    "#             T(n/2)=2T(n/4)+c\n",
    "#Substitute this back into the original equation:\n",
    "\n",
    "#             T(n)=2(2T(n/4+c)+c\n",
    "#Simplify:\n",
    "#             T(n)=4T(n/4)+3c\n",
    "#Third Substitution:\n",
    "#             T(n/4)=2T(n/8)+c\n",
    " #Substitute this into the second substitution:\n",
    "#             T(n)=4(2T(n/8)+c)+3c\n",
    "#Simplify:\n",
    "\n",
    "#             T(n)=8T(n/8)+7c\n",
    "\n",
    "#After k steps, we get:\n",
    "#            T(n)=2T(n/2k)+kc\n",
    "\n",
    "#now, we need to find the value of k when n/2k = 1, which gives us k=log2n.\n",
    "\n",
    "#Substitute k=log2n into the expression: \n",
    "             #T(n)= 2log2nT(1) + log2n.c\n",
    "\n",
    "#Simplify further using the fact that \n",
    "\n",
    "#             T(n)=nT(1)+log2n.c \n",
    "\n",
    "#If you have an initial condition T(1), you can substitute it in. If not, you can leave the solution in this form.\n"
   ]
  },
  {
   "cell_type": "markdown",
   "metadata": {},
   "source": [
    "2. Given a recurrence relation, solve it using the substitution method:\n",
    "\n",
    "d. T(n) = T(n/2) + c"
   ]
  },
  {
   "cell_type": "code",
   "execution_count": 8,
   "metadata": {},
   "outputs": [],
   "source": [
    "#To solve the recurrence relation T(n) = T(n/2)+c using the substitution method, let's express it in terms of smaller subproblems until we reach the base case.\n",
    "\n",
    "#First Substitution:\n",
    "           #T(n)=T(n/2)+c\n",
    "\n",
    "#Second Substitution:\n",
    "\n",
    "           #T(n/2)=T(n/4)+c\n",
    "#Substitute this back into the original equation:\n",
    "           #T(n)=T(n/4)+2c\n",
    "\n",
    "#Third Substitution:\n",
    "           #T(n/4)=T(n/8)+c\n",
    "#Substitute this into the second substitution:\n",
    "\n",
    "           #T(n)=T(n/8)+3c\n",
    "\n",
    "#After k steps, we get:\n",
    "\n",
    "           #T(n)=T(n/2k)+kc\n",
    "\n",
    "#Now, we need to find the value of k when n/2k=1, which gives us k=log2n.\n",
    "\n",
    "#Substitute k = log2n into the expression:\n",
    "\n",
    "           #T(n)=T(1)+log2n⋅c\n",
    "\n",
    "#If you have an initial condition T(1), you can substitute it in. If not, you can leave the solution in this form. \n",
    "#So, the solution to the recurrence relation T(n)= T(n/2)+c using the substitution method is T(n)= T(1) + log2n.c \n"
   ]
  },
  {
   "cell_type": "markdown",
   "metadata": {},
   "source": [
    "3. Given a recurrence relation, solve it using the recursive tree approach:\n",
    "\n",
    "a. T(n) = 2T(n-1) +1"
   ]
  },
  {
   "cell_type": "code",
   "execution_count": null,
   "metadata": {},
   "outputs": [],
   "source": [
    "#To solve this recurrence relation T(n)=2T(n-1)+1 using the recursive tree approach we can visualize calls as a tree.\n",
    "#Each level of the tree represents a different value of n, and each node represents a subproblem.\n",
    "#the recursive tree for this recurrence relation can be represented as follows:\n",
    "\n",
    "#T(n)\n",
    "#  |\n",
    "# +-- 2T(n-1) + 1\n",
    "#         |\n",
    "#         +-- 2T(n-2) + 1\n",
    "#                |\n",
    "#                +-- 2T(n-3) + 1\n",
    "#                       |\n",
    "#                       +-- ...\n",
    "# Now,let's analyze the strucure of the tree and identify a pattern.\n",
    "\n",
    "#1.First level(n):\n",
    "          # T(n)=2T(n-1)+1\n",
    "\n",
    "#2. Second level(n-1):\n",
    "           # T(n-1)=2T(n-2)+1\n",
    "    #substitute this into the first level:\n",
    "          #T(n)=2(2T(n-2)+1)+1=4T(n-2)+3\n",
    "\n",
    "#3. Third level(n-2):\n",
    "           #T(n-2)=2T(n-3)+1\n",
    "\n",
    "    #substitute this into the second level :\n",
    "           #T(n-1)=2(2T(n-3)+1)+1=4T(n-3)+3\n",
    "    #substitute this into the first level:\n",
    "           #T(n)=2(4T(n-3)+3)+1=8T(n-3)+7\n",
    "   #After k levels, we can generalize the pattern:\n",
    "\n",
    "          #T(n)=2kT(n-k)+(2k-1)\n",
    "\n",
    "#Now, we need to find when n-k=0 to each the base cash. This gives us k = n.\n",
    "\n",
    "   #Substitute k=n into the expression:\n",
    "          #T(n)=2nT(0)+(2n-1)\n",
    "\n",
    "# if you have in initial condition T(0), you can substitute it in. if not, you canm leave the solution in this form. \n",
    "#So,the solution to the recurrence relation T(n)=2T(n-1)+1 using the recursive tree approach is T(n)=2nT(0)+(2n-1),where T(0)is the initial condition.\n",
    "\n",
    "\n"
   ]
  },
  {
   "cell_type": "markdown",
   "metadata": {},
   "source": [
    "3. Given a recurrence relation, solve it using the recursive tree approach:\n",
    "\n",
    "b. T(n) = 2T(n/2) + n"
   ]
  },
  {
   "cell_type": "code",
   "execution_count": null,
   "metadata": {},
   "outputs": [],
   "source": [
    "#To solve this recurrence relation T(n)=2T(n/2)+n using the recursive tree approach we can visualize calls as a tree.\n",
    "#Each level of the tree represents a different value of n, and each node represents a subproblem.\n",
    "#the recursive tree for this recurrence relation can be represented as follows:\n",
    "\n",
    "#T(n)\n",
    "#  |\n",
    "# +-- 2T(n/2) + n\n",
    "#         |\n",
    "#         +-- 2T(n/4) + n/2\n",
    "#                |\n",
    "#                +-- 2T(n/8) + n/4\n",
    "#                       |\n",
    "#                       +-- ...\n",
    "# Now,let's analyze the strucure of the tree and identify a pattern.\n",
    "\n",
    "#1.First level(n):\n",
    "          # T(n)=2T(n/2)+n\n",
    "\n",
    "#2. Second level(n-1):\n",
    "           # T(n/2)=2T(n/4)+n/2\n",
    "    #substitute this into the first level:\n",
    "          #T(n)=2(2T(n/4)+n/2)+n=4T(n/4)+n\n",
    "\n",
    "#3. Third level(n-2):\n",
    "           #T(n/4)=2T(n/8)+n/4\n",
    "\n",
    "    #substitute this into the second level :\n",
    "           #T(n/2)=2(2T(n/8)+n/4)+n/2=4T(n/8)+n/2\n",
    "    #substitute this into the first level:\n",
    "           #T(n)=2(4T(n/8)+n/2)+n=8T(n/8)+n\n",
    "   #After k levels, we can generalize the pattern:\n",
    "\n",
    "          #T(n)=2kT(n/2k)+kn\n",
    "\n",
    "#Now, we need to find when n/2k=1 to each the base cash. This gives us k = log2n.\n",
    "\n",
    "   #Substitute k=log2n into the expression:\n",
    "          #T(n)=2log2nT(1)+nlog2n\n",
    "\n",
    "#simplify k = log2n into the expression:\n",
    "           #T(n)=2log2nt(1)+nlog2nS\n",
    "\n",
    "# if you have in initial condition T(0), you can substitute it in. if not, you canm leave the solution in this form. \n",
    "#So,the solution to the recurrence relation T(n)=2T(n-1)+1 using the recursive tree approach is T(n)=2nT(0)+(2n-1),where T(0)is the initial condition.\n",
    "\n",
    "\n"
   ]
  }
 ],
 "metadata": {
  "kernelspec": {
   "display_name": "Python 3",
   "language": "python",
   "name": "python3"
  },
  "language_info": {
   "codemirror_mode": {
    "name": "ipython",
    "version": 3
   },
   "file_extension": ".py",
   "mimetype": "text/x-python",
   "name": "python",
   "nbconvert_exporter": "python",
   "pygments_lexer": "ipython3",
   "version": "3.11.6"
  }
 },
 "nbformat": 4,
 "nbformat_minor": 2
}
